Coalesce some fupds to make is_proposal_valid simpler; will need to
use later credits or something to deal with the fact that we might open
an arbitrarily large number invariants, and fire fupd from each of them
when committing something. Each fupd will have a later because of the
invariant, and so we could have a ~(num entries in the log) laters.

Prove ghost_commit; reprove ghost_commit except for this later trouble.

src/program_proof/simplepb/pb_definitions.v
@@ -81,22 +81,27 @@ Definition old_proposal_max γ epoch σ : iProp Σ := (* persistent *)
    committed_by γ epoch_old σ_old → ⌜σ_old ⪯ σ⌝).
 
 Definition pbN := nroot .@ "pb".
+Definition sysN := pbN .@ "sys".
+Definition opN := pbN .@ "op".
 
-Definition is_valid_inv γ epoch σ op : iProp Σ :=
-  inv pbN (
-    (|={⊤,∅}=> ∃ someσ, own_ghost γ someσ ∗ (⌜someσ = σ⌝ -∗ own_ghost γ (someσ ++ [op]) ={∅,⊤}=∗ True)) ∨
+Definition is_valid_inv γ σ op : iProp Σ :=
+  inv opN (
+    (|={⊤∖↑pbN,∅}=> ∃ someσ, own_ghost γ someσ ∗ (⌜someσ = σ⌝ -∗ own_ghost γ (someσ ++ [op]) ={∅,⊤∖↑pbN}=∗ True)) ∨
     is_ghost_lb γ (σ ++ [op])
   )
 .
 
-Definition is_proposal_valid γ epoch σ : iProp Σ :=
+Definition is_proposal_valid_old γ σ : iProp Σ :=
   ∀ σprev op σnext,
   ⌜σ = σprev ++ [op] ++ σnext⌝ -∗
-  is_valid_inv γ epoch σprev op.
+  is_valid_inv γ σprev op.
+
+Definition is_proposal_valid γ σ : iProp Σ :=
+  □(∀ σ', ⌜σ' ⪯ σ⌝ → own_commit γ σ' ={⊤∖↑sysN}=∗ own_commit γ σ).
 
 Definition is_proposal_facts γ epoch σ: iProp Σ :=
   old_proposal_max γ epoch σ ∗
-  is_proposal_valid γ epoch σ.
+  is_proposal_valid γ σ.
 
 Definition own_Server_ghost γ epoch σ : iProp Σ :=
   "Hepoch_ghost" ∷ own_epoch γ epoch ∗
@@ -175,10 +180,10 @@ Qed.
 Lemma ghost_propose γ epoch σ op :
   own_proposal γ epoch σ -∗
   is_proposal_facts γ epoch σ -∗
-  (|={⊤,∅}=> ∃ someσ, own_ghost γ someσ ∗ (⌜someσ = σ⌝ -∗ own_ghost γ (someσ ++ [op]) ={∅,⊤}=∗ True))
+  (|={⊤∖↑pbN,∅}=> ∃ someσ, own_ghost γ someσ ∗ (⌜someσ = σ⌝ -∗ own_ghost γ (someσ ++ [op]) ={∅,⊤∖↑pbN}=∗ True))
   ={⊤}=∗
   own_proposal γ epoch (σ ++ [op]) ∗
-  is_proposal_facts γ epoch (σ ++ [op]).
+  (▷ is_proposal_facts γ epoch (σ ++ [op])).
 Proof.
   iIntros "Hprop #Hprop_facts Hupd".
   iSplitL "Hprop".
@@ -196,6 +201,7 @@ Proof.
     iModIntro.
     unfold old_proposal_max.
     iModIntro.
+    iModIntro.
     iIntros.
     iAssert (⌜σ_old ⪯ σ⌝)%I as "%Hprefix".
     {
@@ -212,7 +218,7 @@ Proof.
   iDestruct "Hprop_facts" as "[_ #Hvalid]".
   unfold is_proposal_valid.
 
-  iAssert (|={⊤}=> is_valid_inv γ epoch σ op)%I with "[Hupd]" as ">#Hinv".
+  iAssert (|={⊤}=> is_valid_inv γ σ op)%I with "[Hupd]" as ">#Hinv".
   {
     iMod (inv_alloc with "[Hupd]") as "$".
     {
@@ -221,47 +227,114 @@ Proof.
     }
     done.
   }
+  (* prove is_proposal_valid γ (σ ++ [op]) *)
   iModIntro.
-  iIntros (σprev op_some σnext Hσ).
-  assert (length σnext = 0 ∨ length σnext > 0) as Hineqs by lia.
-  destruct Hineqs as [Hineq | Hineq].
-  {
-    rewrite length_zero_iff_nil in Hineq.
-    rewrite Hineq in Hσ.
-    simpl in Hσ.
-    assert (op = op_some) as ->.
-    { (* TODO: list_solver *)
-      apply (f_equal last) in Hσ.
-      rewrite last_snoc in Hσ.
-      rewrite last_snoc in Hσ.
-      naive_solver.
-    }
-    apply app_inv_tail in Hσ.
-    rewrite Hσ.
-    iFrame "Hinv".
-  }
-  {
-    assert (σ = σprev ++ [op_some] ++ removelast σnext) as H.
+  iModIntro.
+  iModIntro.
+  iIntros (σ') "%Hσ' Hσ'".
+  assert (σ' ⪯ σ ∨ σ' = (σ ++ [op])) as [Hprefix_old|Hlatest].
+  { (* TODO: list_solver. *)
+    Search prefix.
+    assert (Hlen := Hσ').
+    apply prefix_length in Hlen.
+    assert (length σ' = length (σ ++ [op]) ∨ length σ' < length (σ ++ [op])) as [|] by word.
     {
-      (* TODO: list_solver *)
-      assert (removelast (σ ++ [op]) = removelast (σprev ++ [op_some] ++ σnext)).
-      { by rewrite Hσ. }
-      rewrite removelast_last in H.
-      rewrite removelast_app in H; last first.
-      { done. }
-      rewrite removelast_app in H; last first.
-      { by apply length_nonzero_neq_nil. }
-      done.
+      right.
+      apply list_prefix_eq; eauto.
+      lia.
     }
-    iApply "Hvalid".
-    done.
+    {
+      left.
+      rewrite app_length in H.
+      simpl in H.
+      apply list_prefix_bounded.
+      { word. }
+      intros.
+      assert (σ !! i = (σ ++ [op]) !! i).
+      {
+        rewrite lookup_app_l.
+        { done. }
+        { word. }
+      }
+      rewrite H1.
+      apply list_prefix_forall.
+      { done. }
+      { done. }
+    }
   }
-Qed.
+  {
+    iMod ("Hvalid" $! σ' Hprefix_old with "Hσ'") as "Hσ".
+    iInv "Hinv" as "Hi" "Hclose".
+    iDestruct "Hi" as "[Hupd|#>Hlb]"; last first.
+    {
+      iDestruct (own_valid_2 with "Hσ Hlb") as "%Hvalid".
+      exfalso.
+      rewrite mono_list_both_dfrac_valid_L in Hvalid.
+      destruct Hvalid as [_ Hvalid].
+      apply prefix_length in Hvalid.
+      rewrite app_length in Hvalid.
+      simpl in Hvalid.
+      word.
+    }
+    iAssert (|={⊤ ∖ ↑pbN,∅}=>
+                ∃ someσ : list EntryType, own_ghost γ someσ ∗
+                  (⌜someσ = σ⌝ -∗ own_ghost γ (someσ ++ [op]) ={∅,⊤ ∖ ↑pbN}=∗ True))%I
+            with "[Hupd]" as "Hupd".
+    { (* FIXME: need to strip off this later *)
+      admit.
+    }
+    iMod (fupd_mask_subseteq (⊤∖↑pbN)) as "Hmask".
+    {
+      assert ((↑sysN:coPset) ⊆ (↑pbN:coPset)).
+      { apply nclose_subseteq. }
+      assert ((↑opN:coPset) ⊆ (↑pbN:coPset)).
+      { apply nclose_subseteq. }
+      set_solver.
+    }
+    iMod "Hupd".
+    iDestruct "Hupd" as (?) "[Hghost Hupd]".
+    iDestruct (own_valid_2 with "Hghost Hσ") as %Hvalid.
+    rewrite mono_list_auth_dfrac_op_valid_L in Hvalid.
+    destruct Hvalid as [_ ->].
+    iCombine "Hghost Hσ" as "Hσ".
+    rewrite -mono_list_auth_dfrac_op.
+    rewrite dfrac_op_own.
+    rewrite Qp_half_half.
+    iMod (own_update with "Hσ") as "Hσ".
+    {
+      apply (mono_list_update (σ ++ [op] : list (leibnizO EntryType))).
+      by apply prefix_app_r.
+    }
+    iEval (rewrite -Qp_half_half) in "Hσ".
+    rewrite -dfrac_op_own.
+    rewrite mono_list_auth_dfrac_op.
+    iDestruct "Hσ" as "[Hσ Hcommit]".
+    iSpecialize ("Hupd" with "[] Hσ").
+    { done. }
+    iMod "Hupd".
 
-Definition sys_inv γ := inv pbN
+    rewrite mono_list_auth_lb_op.
+    iDestruct "Hcommit" as "[Hcommit #Hlb]".
+    iMod "Hmask".
+    iMod ("Hclose" with "[]").
+    {
+      iNext.
+      iRight.
+      iFrame "Hlb".
+    }
+    iModIntro.
+    iFrame.
+  }
+  {
+    rewrite Hlatest.
+    by iFrame.
+  }
+Admitted.
+
+Definition sys_inv γ := inv sysN
 (
   ∃ σ epoch,
-  own_ghost γ σ ∗
+  own_commit γ σ ∗
   committed_by γ epoch σ ∗
   is_proposal_lb γ epoch σ ∗
   is_proposal_facts γ epoch σ
@@ -307,11 +380,24 @@ Proof.
 
   destruct Hlog as [Hcan_update|Halready_updated].
   {
-    (* TODO: need to fire a bunch of fupds *)
-    admit.
+    iEval (unfold is_proposal_valid) in "Hvalid".
+    iDestruct ("Hvalid" $! σcommit with "[] Hghost") as "Hghost".
+    { done. }
+    iMod "Hghost".
+    unfold own_commit.
+    iEval (rewrite mono_list_auth_lb_op) in "Hghost".
+    iDestruct "Hghost" as "[Hghost $]".
+    iMod ("Hclose" with "[-]").
+    {
+      iNext.
+      iExists _, _. iFrame "∗".
+      iFrame "Hcom".
+      iFrame "#".
+    }
+    done.
   }
   {
-    unfold own_ghost.
+    unfold own_commit.
     iEval (rewrite mono_list_auth_lb_op) in "Hghost".
     iDestruct "Hghost" as "[Hghost #Hlb]".
     iDestruct (own_mono with "Hlb") as "$".
@@ -325,7 +411,7 @@ Proof.
     }
     done.
   }
-Admitted.
+Qed.
 
 End pb_protocol.
 
